DependentComputability/Bare.lean
@@ -1,0 +1,217 @@
+import DependentComputability.NewDecls
+
+def Bare (α : Sort u) := α
+def Bare.mk {α : Sort u} (a : α) : Bare α := a
+
+def _root_.New.Bare : new_type% @Bare.{u} :=
+  fun _ _ => .mk (fun _ => PUnit) (TrivialEncoding _) (.trivialEncoding _)
+
+def New.Bare.mk : new_type% @Bare.mk.{u} :=
+  fun _ _ _ _ => ⟨⟩
+
+class BareSurj (α : Sort u) where
+  ofBare : Bare α → α
+  mk_ofBare (x : Bare α) : Bare.mk (ofBare x) = x
+
+def Bare.value [BareSurj α] (x : Bare α) : α := BareSurj.ofBare x
+
+@[simp]
+lemma Bare.mk_value [BareSurj α] (x : Bare α) : mk x.value = x :=
+  BareSurj.mk_ofBare x
+
+lemma Bare.mk_surjective [BareSurj α] : (mk (α := α)).Surjective := by
+  intro x; use x.value; exact x.mk_value
+
+lemma Bare.value_injective [BareSurj α] : (value (α := α)).Injective := by
+  intro x y h
+  rw [← mk_value x, ← mk_value y, h]
+
+@[simp]
+lemma Bare.value_inj [BareSurj α] {x y : Bare α} :
+    x.value = y.value ↔ x = y := value_injective.eq_iff
+
+class BareInj (α : Sort u) where
+  mk_injective : (Bare.mk (α := α)).Injective
+
+lemma Bare.mk_injective [BareInj α] : (mk (α := α)).Injective :=
+  BareInj.mk_injective
+
+@[simp]
+lemma Bare.mk_inj [BareInj α] {x y : α} : mk x = mk y ↔ x = y :=
+  mk_injective.eq_iff
+
+@[simp]
+lemma Bare.value_mk [BareSurj α] [BareInj α] (x : α) : (mk x).value = x := by
+  apply mk_injective; simp
+
+def BareSurj.unsafeIntro : BareSurj α where
+  ofBare x := x
+  mk_ofBare _ := rfl
+
+def BareInj.unsafeIntro : BareInj α where
+  mk_injective := Function.injective_id
+
+def bareSurj_of_inhabitedExtra [@InhabitedExtra α α'] :
+    (new% BareSurj α).1 .unsafeIntro :=
+  .mk _ _ (fun _ _ => InhabitedExtra.default _) (fun _ _ => .refl _)
+
+@[implicit_reducible]
+def inhabitedExtra_of_bareSurj {α : Sort u} {α' : new_type% α}
+    {h : BareSurj α} (h' : new_type% h) : InhabitedExtra α' where
+  default x := h.2 x ▸ @h'.1 x ⟨⟩
+
+lemma bareInj_of_subsingletonExtra [@SubsingletonExtra α α'] :
+    (new% BareInj α).1 .unsafeIntro := by
+  constructor
+  intro a a' b b' h h'
+  cases h
+  cases Subsingleton.allEq a' b'
+  constructor
+
+lemma subsingletonExtra_of_bareInj {α : Sort u} {α' : new_type% α}
+    {h : BareInj α} (h' : new_type% h) : SubsingletonExtra α' where
+  subsingleton x := {
+    allEq a b := by
+      cases @h'.1 x a x b rfl (.refl _)
+      rfl
+  }
+
+@[simp]
+lemma Bare.eq_iff : Bare (a = b) ↔ Bare.mk a = Bare.mk b := Iff.rfl
+
+instance {α : Sort u} {α' : new_type% α} : InhabitedExtra (new% Bare α) where
+  default _ := ⟨⟩
+
+instance {α : Sort u} {α' : new_type% α} : SubsingletonExtra (new% Bare α) where
+  subsingleton _ := inferInstanceAs (Subsingleton PUnit)
+
+instance {a b : α} [BareInj α] : BareSurj (a = b) where
+  ofBare := by simp
+  mk_ofBare _ := rfl
+
+instance : InhabitedExtra (new% PUnit.{u}) where
+  default _ := ⟨⟩
+
+instance : SubsingletonExtra (new% PUnit.{u}) where
+  subsingleton _ := inferInstanceAs (Subsingleton PUnit)
+
+instance : InhabitedExtra (new% Bool) where
+  default := by rintro ⟨⟩ <;> constructor
+
+instance : SubsingletonExtra (new% Bool) where
+  subsingleton _ := by constructor; rintro ⟨⟩ ⟨⟩ <;> constructor
+
+instance : InhabitedExtra (new% Nat) where
+  default _ := ⟨⟩
+
+instance : SubsingletonExtra (new% Nat) where
+  subsingleton _ := by constructor; intros; rfl
+
+instance : InhabitedExtra (new% True) where
+  default := by rintro ⟨⟩; constructor
+
+instance : InhabitedExtra (new% False) where
+  default := nofun
+
+instance instBareSurjPUnit : BareSurj PUnit := .unsafeIntro
+instance instBareInjPUnit : BareInj PUnit := .unsafeIntro
+instance instBareSurjBool : BareSurj Bool := .unsafeIntro
+instance instBareInjBool : BareInj Bool := .unsafeIntro
+instance instBareSurjNat : BareSurj Nat := .unsafeIntro
+instance instBareInjNat : BareInj Nat := .unsafeIntro
+instance instBareSurjTrue : BareSurj True := .unsafeIntro
+instance instBareSurjFalse : BareSurj False := .unsafeIntro
+
+def New.instBareSurjPUnit : new_type% @instBareSurjPUnit.{u} := bareSurj_of_inhabitedExtra
+def New.instBareInjPUnit : new_type% @instBareInjPUnit.{u} := bareInj_of_subsingletonExtra
+def New.instBareSurjBool : new_type% @instBareSurjBool := bareSurj_of_inhabitedExtra
+def New.instBareInjBool : new_type% @instBareInjBool := bareInj_of_subsingletonExtra
+def New.instBareSurjNat : new_type% @instBareSurjNat := bareSurj_of_inhabitedExtra
+def New.instBareInjNat : new_type% @instBareInjNat := bareInj_of_subsingletonExtra
+def New.instBareSurjTrue : new_type% @instBareSurjTrue := bareSurj_of_inhabitedExtra
+def New.instBareSurjFalse : new_type% @instBareSurjFalse := bareSurj_of_inhabitedExtra
+
+instance {α : Sort u} {α' : new_type% α} {p : α → Prop} {p' : new_type% p}
+    [InhabitedExtra α'] [∀ a a', InhabitedExtra (@p' a a')] :
+    InhabitedExtra (new% Exists p) where
+  default | ⟨x, h⟩ => ⟨InhabitedExtra.default x, InhabitedExtra.default h⟩
+
+instance instBareSurjExists {α : Sort u} {p : α → Prop} [BareSurj α]
+    [∀ a, BareSurj (p a)] : BareSurj (Exists p) := .unsafeIntro
+
+def New.instBareSurjExists : new_type% @instBareSurjExists.{u} :=
+  fun _ _ _ _ _ hα' _ hp' =>
+    let := inhabitedExtra_of_bareSurj hα'
+    let (a a' : _) := inhabitedExtra_of_bareSurj (@hp' a a')
+    bareSurj_of_inhabitedExtra
+
+instance {α : Sort u} {α' : new_type% α} {r : α → α → Prop} {r' : new_type% r}
+    [InhabitedExtra α'] [∀ a a' b b', InhabitedExtra (@r' a a' b b')] :
+    InhabitedExtra (new% Quot r) where
+  default x := by
+    refine x.rec ?_ ?_
+    · intro x
+      refine Quot.mk _ ?_
+      constructor
+      exact InhabitedExtra.default x
+    · intro a b h
+      rw! (castMode := .all) [Quot.sound h]
+      apply Quot.sound
+      let : new_type% a := InhabitedExtra.default _
+      let : new_type% b := InhabitedExtra.default _
+      let : new_type% h := InhabitedExtra.default _
+      exact .mk (new% a) (new% b) (new% h)
+
+instance {α : Sort u} {α' : new_type% α} {r : α → α → Prop} {r' : new_type% r}
+    [InhabitedExtra α'] [SubsingletonExtra α'] [∀ a a' b b', InhabitedExtra (@r' a a' b b')] :
+    SubsingletonExtra (new% Quot r) where
+  subsingleton x := by
+    constructor
+    rintro ⟨a⟩ ⟨b⟩
+    have := 0
+    clear ‹new_type% x›
+    clear ‹new_type% x›
+    rcases a with @⟨a, a'⟩
+    have (eq := q_eq) q := Quot.mk r a
+    revert b
+    rw! (castMode := .all) [← q_eq]
+    rintro @⟨b, b'⟩
+    revert q_eq
+    rw! [eq_comm, Iff.intro Quot.eqvGen_exact Quot.eqvGen_sound]
+    intro q_eq
+    induction q_eq with
+    | rel a b h =>
+      apply Quot.sound
+      have : new_type% h := InhabitedExtra.default h
+      exact .mk (new% a) (new% b) (new% h)
+    | refl a => cases Subsingleton.allEq a' b'; rfl
+    | symm a b h ih =>
+      specialize ih b' a'
+      rw! (castMode := .all) [Quot.eqvGen_sound h]
+      exact ih.symm
+    | trans a b c h h' ih ih' =>
+      rename' b' => c'
+      let b' : new_type% b := InhabitedExtra.default b
+      specialize ih a' b'
+      specialize ih' b' c'
+      rw! (castMode := .all) [Quot.eqvGen_sound h'] at ih
+      exact ih.trans ih'
+
+instance instBareSurjQuot {α : Sort u} {r : α → α → Prop} [BareSurj α]
+    [∀ a b, BareSurj (r a b)] : BareSurj (Quot r) := .unsafeIntro
+
+instance instBareInjQuot {α : Sort u} {r : α → α → Prop} [BareSurj α] [BareInj α]
+    [∀ a b, BareSurj (r a b)] : BareInj (Quot r) := .unsafeIntro
+
+def New.instBareSurjQuot : new_type% @instBareSurjQuot.{u} :=
+  fun _ _ _ _ _ hα' _ hr' =>
+    let := inhabitedExtra_of_bareSurj hα'
+    let (a a' b b' : _) := inhabitedExtra_of_bareSurj (@hr' a a' b b')
+    bareSurj_of_inhabitedExtra
+
+def New.instBareInjQuot : new_type% @instBareInjQuot.{u} :=
+  fun _ _ _ _ _ hα' _ hα₂' _ hr' =>
+    let := inhabitedExtra_of_bareSurj hα'
+    let := subsingletonExtra_of_bareInj hα₂'
+    let (a a' b b' : _) := inhabitedExtra_of_bareSurj (@hr' a a' b b')
+    bareInj_of_subsingletonExtra
